code/experimental/ed25519/Hacl.Impl.Ed25519.Sign.Steps.fst
@@ -84,7 +84,8 @@ val sign_step_2:
       disjoint tmp_bytes msg /\ disjoint tmp_bytes tmp_ints /\
       disjoint tmp_ints msg)
     (ensures fun h0 _ h1 -> modifies (loc tmp_ints) h0 h1 /\
-      F56.fevalh h1 (gsub tmp_ints 20ul 5ul) == Spec.Ed25519.sha512_modq (32 + v len)
+      F56.as_nat h1 (gsub tmp_ints 20ul 5ul) < pow2 256 /\
+      F56.as_nat h1 (gsub tmp_ints 20ul 5ul) == Spec.Ed25519.sha512_modq (32 + v len)
         (concat #uint8 #32 #(v len) (as_seq h0 (gsub tmp_bytes 256ul 32ul)) (as_seq h0 msg)))
 
 let sign_step_2 len msg tmp_bytes tmp_ints =
@@ -93,14 +94,17 @@ let sign_step_2 len msg tmp_bytes tmp_ints =
   let apre   = sub tmp_bytes 224ul 64ul in
   let a      = sub apre 0ul 32ul in
   let prefix = sub apre 32ul 32ul in
-  Hacl.Impl.SHA512.ModQ.sha512_modq_pre r prefix len msg
+  Hacl.Impl.SHA512.ModQ.sha512_modq_pre r prefix len msg;
+  assert_norm (Spec.Ed25519.q < pow2 256)
 
 val sign_step_3:
     tmp_bytes:lbuffer uint8 352ul
   -> tmp_ints:lbuffer uint64 65ul ->
   Stack unit
     (requires fun h ->
-      live h tmp_bytes /\ live h tmp_ints /\ disjoint tmp_bytes tmp_ints)
+      live h tmp_bytes /\ live h tmp_ints /\ disjoint tmp_bytes tmp_ints /\
+      F56.as_nat h (gsub tmp_ints 20ul 5ul) < pow2 256
+    )
     (ensures fun h0 _ h1 -> modifies (loc tmp_bytes) h0 h1 /\
       // Framing
       as_seq h0 (gsub tmp_bytes 96ul 32ul) == as_seq h1 (gsub tmp_bytes 96ul 32ul) /\
@@ -108,7 +112,7 @@ val sign_step_3:
       // Postcondition
       as_seq h1 (gsub tmp_bytes 160ul 32ul) ==
       Spec.Ed25519.point_compress (Spec.Ed25519.point_mul
-        (nat_to_bytes_le 32 (F56.fevalh h0 (gsub tmp_ints 20ul 5ul)))
+        (nat_to_bytes_le 32 (F56.as_nat h0 (gsub tmp_ints 20ul 5ul)))
         (Spec.Ed25519.g)))
 
 let sign_step_3 tmp_bytes tmp_ints =
@@ -139,7 +143,7 @@ val sign_step_4:
       // Framing
       as_seq h0 (gsub tmp_ints 20ul 5ul) == as_seq h1 (gsub tmp_ints 20ul 5ul) /\
       // Postcondition
-      F56.fevalh h1 (gsub tmp_ints 60ul 5ul) ==
+      F56.as_nat h1 (gsub tmp_ints 60ul 5ul) ==
       Spec.Ed25519.sha512_modq (64 + v len)
         (concat #uint8 #64 #(v len)
           (concat #uint8 #32 #32
@@ -170,8 +174,8 @@ val sign_step_5:
       // Framing
       as_seq h0 (gsub tmp_bytes 160ul 32ul) == as_seq h1 (gsub tmp_bytes 160ul 32ul) /\
       // Postcondition
-      (let r = F56.fevalh h0 (gsub tmp_ints 20ul 5ul) in
-       let h = F56.fevalh h0 (gsub tmp_ints 60ul 5ul) in
+      (let r = F56.as_nat h0 (gsub tmp_ints 20ul 5ul) in
+       let h = F56.as_nat h0 (gsub tmp_ints 60ul 5ul) in
        let a = as_seq h0 (gsub tmp_bytes 224ul 32ul) in
       nat_from_bytes_le (as_seq h1 (gsub tmp_bytes 192ul 32ul)) ==
       (r + (h * nat_from_bytes_le a) % Spec.Ed25519.q) % Spec.Ed25519.q))
